x=4{0<y<6}

y=4{2<x<6,17<x<18,28<x<30,41<x<42}

y=6{4<x<6,15<x<16,17<x<19,41<x<43,50<x<51}

x=7{0<y<6}

(x-9)^2+(y-3)^2=1

x=10{2<y<3}

(x-12)^2+(y-3)^2=1

x=13{0<y<3}

y=0{11<x<13,15<x<16,50<x<51}

y=-x+17{14<x<15}

y=x-11{14<x<15}

x=15{0<y<2,4<y<6}

x=17{1<y<6}

x=19{3<y<4}

x=21{3<y<4}

(x-20)^2+(y-3)^2=1{2<y<3}

(x-23)^2+(y-3)^2=1{3<y<4}

x=22{2<y<3}

x=24{2<y<3}

(x-26)^2+(y-3)^2=1{25<x<26}

y=0.5x-11{26<x<27}

y=-0.5x+17{26<x<27}

y=2{29<x<30,31<x<33,39<x<40}

x=29{2<y<5}

x=32{2<y<5}

y=x-27{31<x<32}

(x-34)^2+((y-3.5)^2)/(1.5^2)=1

x=36{2<y<3}

(x-37)^2+(y-3)^2=1{3<y<4}

x=38{2<y<3}

x=41{2<y<6}

x=44{3<y<4}

(x-45)^2+(y-3)^2=1{2<y<3}

x=46{3<y<4}

x=47{2<y<3}

(x-48)^2+(y-3)^2=1{3<y<4}

x=49{2<y<3}

x=51{0<y<2,4<y<6}

y=x-49{51<x<52}

y=-x+55{51<x<52}